dq-checkers/rocq/theories/ClassBalance.v
@@ -1,6 +1,7 @@
 From Coq Require Import
      Arith
-     Bool.
+     Bool
+     PeanoNat.
 
 Open Scope nat_scope.
 
@@ -11,6 +12,7 @@ Open Scope nat_scope.
 
 Module ClassBalanceAtom.
 
+  (* Absolute difference on nat *)
   Definition nat_abs (n m : nat) : nat :=
     if Nat.leb n m then m - n else n - m.
 
@@ -18,14 +20,16 @@ Module ClassBalanceAtom.
   Definition within_tolerance (exp obs tol : nat) : bool :=
     Nat.leb (nat_abs exp obs) tol.
 
-  (* Logical spec skeleton, for later proof *)
+  (* Logical spec: absolute deviation is bounded by tol *)
   Definition within_toleranceP (exp obs tol : nat) : Prop :=
-    (Nat.leb (nat_abs exp obs) tol = true).
+    nat_abs exp obs <= tol.
 
   Lemma within_tolerance_spec (exp obs tol : nat) :
     within_tolerance exp obs tol = true <-> within_toleranceP exp obs tol.
   Proof.
-    (* To be refined later; currently just a placeholder. *)
-  Admitted.
+    unfold within_tolerance, within_toleranceP.
+    (* Nat.leb_le: Nat.leb a b = true <-> a <= b *)
+    now rewrite Nat.leb_le.
+  Qed.
 
 End ClassBalanceAtom.
